keep the Pre and unpack pure

theory/System/PathORAM_typeclass.v
@@ -449,6 +449,8 @@ Definition get_stash {n l : nat} : Poram_st (state n l) dist (stash n) :=
 
 Definition get_oram {n l : nat} : Poram_st (state n l) dist (oram n l) :=
   fun s => mreturn(state_oram s,s).
+
+
   
 Fixpoint lookup_path_oram {n l : nat} : forall (p : path l) (o : oram n l), Vector.t (bucket n) l :=
   match l with
@@ -463,6 +465,7 @@ Fixpoint lookup_path_oram {n l : nat} : forall (p : path l) (o : oram n l), Vect
   end.
 #[global] Instance PoramM {S M } `{Monad M} : Monad (Poram_st S M) := {|mreturn A := retT; mbind X Y := bindT  |}.
 
+Definition get_State {n l : nat} : Poram_st(state n l) dist(state n l) := Poram_st_get.
 
 Inductive operation := 
   | Read : operation 
@@ -562,11 +565,16 @@ Definition access_helper {n l : nat} (id : block_id) (op : operation) (m : posit
   (n_st, ret_data).
   
 Definition access {n l : nat} (id : block_id) (op : operation) :
-  Poram_st (state n l) dist (path l * nat) := 
+  Poram_st (state n l) dist (path l * nat) :=
+  PST <- get_State ;;
   (* unpack the state *)
-  m <- get_pos_map ;;
-  h <- get_stash ;;
-  o <- get_oram ;;
+  let m := state_position_map PST in
+  let h := state_stash  PST in
+  let o := state_oram PST in 
+
+  (* m <- get_pos_map ;; *)
+  (* h <- get_stash ;; *)
+  (* o <- get_oram ;; *)
   (* get path for the index we are querying *)
   let p := lookup_dict dummy_path id m in
   (* flip a bunch of coins to get the new path *)      
@@ -691,9 +699,18 @@ Admitted.
 
 (* TODO: having a lemma about get_pos_map is too speicific, find a way to formalize the get lemma that's genenral enough that can be applied to the other get operations  *)
 
-Lemma get_pos_map_wf {n l : nat} {Pre : state n l -> Prop} :
-  state_prob_lift Pre Pre (fun _ => True) get_pos_map. 
+Lemma get_State_wf {n l : nat} {Pre : state n l -> Prop} :
+  state_prob_lift Pre Pre Pre get_State.
 Admitted.
+
+Lemma get_pos_map_wf {n l : nat} {Pre : state n l -> Prop} :
+  state_prob_lift Pre Pre (fun _ => True) get_pos_map.
+Admitted.
+
+(* Lemma get_pos_map_wf {n l : nat} {Pre : state n l -> Prop} {P : position_map l -> Prop} : *)
+(*   (forall s, Pre s -> P (state_position_map s)) -> *)
+(*   state_prob_lift Pre Pre P get_pos_map. *)
+(* Admitted. *)
 
 Lemma get_stash_wf {n l : nat} {Pre : state n l -> Prop}:
   state_prob_lift Pre Pre (fun _ => True) get_stash.
@@ -739,34 +756,32 @@ Lemma zero_sum_stsh_tr_Wr {n l : nat} (id : block_id) (v : nat) (m : position_ma
 Admitted.    
 
 Lemma zero_sum_stsh_tr_Rd {n l : nat} (id : block_id) (v : nat) (m : position_map l) (h : stash n) (o : oram n l) (p : path l)  (p_new : path l):
-  forall (nst : state n l) (ret_data : nat),
+  forall (nst : state n l),
     kv_rel id v (State m h o) -> 
     access_helper id Read m h o p p_new = (nst, v).
 Admitted.    
-                        
+
+
 Lemma read_access_wf {n l : nat}(id : block_id)(v : nat) :
   state_prob_lift (fun st => @well_formed n l st /\ kv_rel id v st) (fun st => @well_formed n l st /\ kv_rel id v st) (has_value v) (read_access id).
 Proof.
   remember (fun st : state n l => well_formed st /\ kv_rel id v st) as Inv. 
-  apply (state_prob_bind Inv (fun _ => True)).
-  - apply get_pos_map_wf.
+  apply (state_prob_bind Inv Inv).
+  - apply get_State_wf.
   - intros.
     apply (state_prob_bind Inv (fun _ => True)).
-    + apply get_stash_wf.
-    + intros. 
+    * apply coin_flip_wf.
+    * intros. destruct access_helper eqn :?. simpl.
       apply (state_prob_bind Inv (fun _ => True)).
-      * apply get_oram_wf.
-      * intros.
-        apply (state_prob_bind Inv (fun _ => True)).
-        -- apply coin_flip_wf.
-        -- intros.
-           destruct (access_helper id Read x x0 x1 (lookup_dict dummy_path id x) x2) eqn:?. simpl.
-           apply (state_prob_bind (fun st : state n l => kv_rel id n0 st)(fun _ => True)).
-           ++ apply put_wf. 
-              admit.           (* need to prove well-formedness of s and kv_rel holds  *) 
-           ++ intros. rewrite HeqInv.
-              admit.           (* need a retT lemma here *)
-Admitted.
+      ++ apply put_wf.
+         admit.                 (* needs a lemma going from kv_rel -> Inv *)
+      ++ intros. rewrite HeqInv. apply state_prob_ret. rewrite HeqInv in H. destruct H. simpl.
+         rewrite zero_sum_stsh_tr_Rd with (v := v) (nst := s) in Heqp.
+         inversion Heqp; auto. exact H2.
+Qed.
+
+Print read_access_wf.
+
 
 Lemma write_access_wf {n l: nat}(id : block_id)(v : nat) :
   state_prob_lift (fun st => @well_formed n l st) (fun st => @well_formed n l st /\ kv_rel id v st) (fun _ => True) (write_access id v).
